+++
title = '1-2'
date = 2023-11-19T23:35:21-05:00
displayPublishedDate = false
draft = false
+++

Question: Show that (ğ›¼ + ğ›½) + ğœ† = ğ›¼ + (ğ›½ + ğœ†) for all ğ›¼, ğ›½, ğœ† âˆˆ ğ‚.

Answer: Let $\alpha = a + ib$, $\beta = c + id$ and 
$\lambda = e + if$ be given.

Then, 
$$
(\alpha + \beta) + \lambda = ((a + ib) + (c + id)) + (e + if)
= ((a + c) + e) + i((b + d) + f)
= (a + (c + e)) + i(d + (b + f))
= \alpha + (\beta + \lambda)
$$

Where the middle equalites come from the properties of $\mathbb{R}$.
