+++
title = '1-3'
date = 2023-11-19T23:35:21-05:00
displayPublishedDate = false
draft = false
+++

Question: Show that (𝛼𝛽)𝜆 = 𝛼(𝛽𝜆) for all 𝛼, 𝛽, 𝜆 ∈ 𝐂.

Answer: Let $\alpha = a + ib$, $\beta = c + id$ and 
$\lambda = e + if$ be given.

Then, 
$$
(\alpha + \beta)\lambda = ((a + ib)(c + id))(e + if)
= (ac - bd) + i(ad + bc))(e + if)
= (ace - bde - bdf + bcf) + i(ade + bce + bcf + bde)
= (a + ib)((ce - df) + i(de + cf))
= \alpha (\beta \lambda)
$$

Where the middle equalites come from the properties of $\mathbb{R}$.
